All libraries type-checking. Starting work on interactive proofs.
git-svn-id: https://scm.gforge.inria.fr/svn/easycrypt/branches/modules@2802 4a0602ed-0ddf-4d1e-8465-5e6d797b7344

theories/Word.ec
@@ -1,13 +1,19 @@
 require        Bool.
-require import Bitstring.
+require        Bitstring.
 require import Int.
 
 cnst k: int.
 axiom k_pos: 0 <= k.
 
 clone Bitstring as Word.
-export Bitstring.
+export Word.Bits.
+export Word.
 
-type word = Word.bitstring.
+type word = bitstring.
 
-axiom fixed_length: forall (w:word), Word.length w = k.
+axiom fixed_length: forall (w:word), length w = k.
+
+(* We can now refine the axioms knowing that the length is fixed. *)
+(* This remains to do *)
+require        Array.
+lemma to_array_length: forall w, Array.length (to_array w) = k.
